% shenry
\begin{equation}
{e^{i\theta }} = \cos \theta  + i\sin \theta 
\end{equation}
$
\cos \left( {\alpha  + \beta } \right) + i\sin \left( {\alpha  + \beta } \right) = {e^{i\left( {\alpha  + \beta } \right)}} = {e^{i\alpha }} \cdot {e^{i\beta }} = \left( {\cos a + i\sin \alpha } \right)\left( {\cos \beta  + i\sin \beta } \right)
$
$
= \cos \alpha \cos \beta  - \sin \alpha \sin \beta  + i\left( {\sin \alpha \cos \beta  + \sin \beta \cos \alpha } \right)
$
$
\Rightarrow
$
\begin{equation}
\cos \left( {\alpha  + \beta } \right) = \cos \alpha \cos \beta  - \sin \alpha \sin \beta
\end{equation}
\begin{equation}
\sin \left( {\alpha  + \beta } \right) = \sin \alpha \cos \beta  + \sin \beta \cos \alpha
\end{equation}
