% shenruiy
设点$A\left( {\cos \theta ,\sin \theta } \right)$,$B\left( { - \cos \theta , - \sin \theta } \right)$，$M\left( {x,y} \right)$到直线$x =  - 1$的距离为$r = \left| {x + 1} \right|$得
\begin{equation}
\left\{ {\begin{array}{*{20}{c}}
{{{\left( {x - \cos \theta } \right)}^2} + {{\left( {y - \sin \theta } \right)}^2} = {{\left( {x + 1} \right)}^2}}\\
{{{\left( {x + \cos \theta } \right)}^2} + {{\left( {y + \sin \theta } \right)}^2} = {{\left( {x + 1} \right)}^2}}
\end{array}} \right.
\end{equation}
将上述两式相加，可得
\begin{equation}
{x^2} + {\cos ^2}\theta  + {y^2} + {\sin ^2}\theta  = {x^2} + 2x + 1
\end{equation}
整理得
\begin{equation}
{y^2} = 2x
\end{equation}
即为所求.
