% shenry
\begin{equation}
{e^{i\theta }} = \cos \theta  + i\sin \theta 
\end{equation}
$
\cos \left( {\alpha  + \beta } \right) + i\sin \left( {\alpha  + \beta } \right) = {e^{i\left( {\alpha  + \beta } \right)}} = {e^{i\alpha }} \cdot {e^{i\beta }} = \left( {\cos a + i\sin \alpha } \right)\left( {\cos \beta  + i\sin \beta } \right)
$
$= \cos \alpha \cos \beta  - \sin \alpha \sin \beta  + i\left( {\sin \alpha \cos \beta  + \sin \beta \cos \alpha } \right)
$
$\Rightarrow$
\begin{equation}
\cos \left( {\alpha  + \beta } \right) = \cos \alpha \cos \beta  - \sin \alpha \sin \beta
\end{equation}
\begin{equation}
\sin \left( {\alpha  + \beta } \right) = \sin \alpha \cos \beta  + \sin \beta \cos \alpha
\end{equation}
$
\cos \left( {2\theta } \right) + i\sin \left( {2\theta } \right) = {e^{i\left( {2\theta } \right)}} = {\left( {{e^{i\theta }}} \right)^2} = {\left( {\cos \theta  + i\sin \theta } \right)^2} = {\cos ^2}\theta  - {\sin ^2}\theta  + 2i\sin \theta \cos \theta \Rightarrow
$
\begin{equation}
\sin 2\theta  = 2\sin \theta \cos \theta 
\end{equation}
\begin{equation}
\cos 2\theta  = {\cos ^2}\theta  - {\sin ^2}\theta
\end{equation}
$\cos 2\theta  = {\cos ^2}\theta  - {\sin ^2}\theta  = 1 - 2{\sin ^2}\theta  = 2{\cos ^2}\theta  - 1\Rightarrow$
\begin{equation}
\sin \theta  = \sqrt {\frac{{1 - \cos 2\theta }}{2}} ,\cos \theta  = \sqrt {\frac{{1 + \cos 2\theta }}{2}}
\end{equation}